pcuic/theories/PCUICAst.v
@@ -93,11 +93,6 @@ Inductive constant_entry :=
   [x1:X1;...;xn:Xn].
 *)
 
-Inductive recursivity_kind :=
-  | Finite (* = inductive *)
-  | CoFinite (* = coinductive *)
-  | BiFinite (* = non-recursive, like in "Record" definitions *).
-
 Inductive local_entry : Set :=
 | LocalDef : term -> local_entry (* local let binding *)
 | LocalAssum : term -> local_entry.
@@ -165,6 +160,7 @@ Record one_inductive_body := {
 
 (** See [mutual_inductive_body] from [declarations.ml]. *)
 Record mutual_inductive_body := {
+  ind_finite : recursivity_kind;
   ind_npars : nat;
   ind_params : context;
   ind_bodies : list one_inductive_body ;
