pcuic/theories/PCUICValidity.v
@@ -1,265 +1,270 @@
 From Coq Require Import Bool String List Program BinPos Compare_dec Omega.
-From MetaCoq.Template Require Import utils.
+From MetaCoq.Template Require Import config utils.
 From MetaCoq.PCUIC Require Import PCUICAst PCUICAstUtils PCUICInduction
      PCUICLiftSubst PCUICTyping PCUICWeakeningEnv PCUICWeakening PCUICInversion
      PCUICSubstitution PCUICReduction PCUICCumulativity PCUICGeneration.
 From Equations Require Import Equations.
 Require Import ssreflect.
-Existing Instance config.default_checker_flags.
 
 Derive NoConfusion for term.
 Derive Signature for typing cumul.
 
-Lemma isWfArity_or_Type_lift Σ n Γ ty (isdecl : n <= #|Γ|):
-  wf Σ -> wf_local Σ Γ ->
-  isWfArity_or_Type Σ (skipn n Γ) ty ->
-  isWfArity_or_Type Σ Γ (lift0 n ty).
-Proof.
-  intros wfΣ wfΓ wfty. rewrite <- (firstn_skipn n Γ) in wfΓ |- *.
-  assert (n = #|firstn n Γ|).
-  { rewrite firstn_length_le; auto with arith. }
-  destruct wfty.
-  - red. left. destruct i as [ctx [u [da Hd]]].
-    exists (lift_context n 0 ctx), u. split.
-    1: now rewrite (lift_destArity [] ty n 0) da.
-    eapply All_local_env_app_inv.
-    eapply All_local_env_app in Hd. intuition eauto.
-    rewrite {3}H.
-    clear -wfΣ wfΓ isdecl a b.
-    induction b; rewrite ?lift_context_snoc; econstructor; simpl; auto.
-    + destruct t0 as [u Hu]. exists u. rewrite Nat.add_0_r.
-      unshelve eapply (weakening_typing Σ (skipn n Γ) Γ0 (firstn n Γ) t _ _ _ (tSort u)); eauto with wf.
-      apply All_local_env_app_inv. intuition eauto.
-    + destruct t0 as [u Hu]. exists u. rewrite Nat.add_0_r.
-      unshelve eapply (weakening_typing Σ (skipn n Γ) Γ0 (firstn n Γ) t _ _ _ (tSort u)); eauto with wf.
-      apply All_local_env_app_inv. intuition eauto.
-    + rewrite Nat.add_0_r.
-      unshelve eapply (weakening_typing Σ (skipn n Γ) Γ0 (firstn n Γ) b _ _ _ t); eauto with wf.
-      eapply All_local_env_app_inv. intuition eauto.
-  - right. destruct i as [u Hu]. exists u.
-    rewrite {3}H.
-    unshelve eapply (weakening_typing Σ (skipn n Γ) [] (firstn n Γ) ty _ _ _ (tSort u)); eauto with wf.
-Qed.
+Section Validity.
+  Context `{cf : config.checker_flags}.
 
-Lemma destArity_it_mkProd_or_LetIn ctx ctx' t :
-  destArity ctx (it_mkProd_or_LetIn ctx' t) =
-  destArity (ctx ,,, ctx') t.
-Proof.
-  induction ctx' in ctx, t |- *; simpl; auto.
-  rewrite IHctx'. destruct a as [na [b|] ty]; reflexivity.
-Qed.
+  Lemma isWfArity_or_Type_lift (Σ : global_env_ext) n Γ ty (isdecl : n <= #|Γ|):
+    wf Σ -> wf_local Σ Γ ->
+    isWfArity_or_Type Σ (skipn n Γ) ty ->
+    isWfArity_or_Type Σ Γ (lift0 n ty).
+  Proof.
+    intros wfΣ wfΓ wfty. rewrite <- (firstn_skipn n Γ) in wfΓ |- *.
+    assert (n = #|firstn n Γ|).
+    { rewrite firstn_length_le; auto with arith. }
+    destruct wfty.
+    - red. left. destruct i as [ctx [u [da Hd]]].
+      exists (lift_context n 0 ctx), u. split.
+      1: now rewrite (lift_destArity [] ty n 0) da.
+      eapply All_local_env_app_inv.
+      eapply All_local_env_app in Hd. intuition eauto.
+      rewrite {3}H.
+      clear -wfΣ wfΓ isdecl a b.
+      induction b; rewrite ?lift_context_snoc; econstructor; simpl; auto.
+      + destruct t0 as [u Hu]. exists u. rewrite Nat.add_0_r.
+        unshelve eapply (weakening_typing Σ (skipn n Γ) Γ0 (firstn n Γ) t _ _ _ (tSort u)); eauto with wf.
+        apply All_local_env_app_inv. intuition eauto.
+      + destruct t0 as [u Hu]. exists u. rewrite Nat.add_0_r.
+        unshelve eapply (weakening_typing Σ (skipn n Γ) Γ0 (firstn n Γ) t _ _ _ (tSort u)); eauto with wf.
+        apply All_local_env_app_inv. intuition eauto.
+      + rewrite Nat.add_0_r.
+        unshelve eapply (weakening_typing Σ (skipn n Γ) Γ0 (firstn n Γ) b _ _ _ t); eauto with wf.
+        eapply All_local_env_app_inv. intuition eauto.
+    - right. destruct i as [u Hu]. exists u.
+      rewrite {3}H.
+      unshelve eapply (weakening_typing Σ (skipn n Γ) [] (firstn n Γ) ty _ _ _ (tSort u)); eauto with wf.
+  Qed.
 
-Lemma isWfArity_Sort Σ Γ s : wf_local Σ Γ -> isWfArity typing Σ Γ (tSort s).
-Proof.
-  intros. exists [], s; intuition auto.
-Qed.
-Hint Extern 10 (isWfArity _ _ _ (tSort _)) => apply isWfArity_Sort : pcuic.
+  Lemma destArity_it_mkProd_or_LetIn ctx ctx' t :
+    destArity ctx (it_mkProd_or_LetIn ctx' t) =
+    destArity (ctx ,,, ctx') t.
+  Proof.
+    induction ctx' in ctx, t |- *; simpl; auto.
+    rewrite IHctx'. destruct a as [na [b|] ty]; reflexivity.
+  Qed.
 
-Hint Extern 30 (wf_local ?Σ ?Γ) =>
+  Lemma isWfArity_Sort Σ Γ s : wf_local Σ Γ -> isWfArity typing Σ Γ (tSort s).
+  Proof.
+    intros. exists [], s; intuition auto.
+  Qed.
+  Hint Extern 10 (isWfArity _ _ _ (tSort _)) => apply isWfArity_Sort : pcuic.
+
+  Hint Extern 30 (wf_local ?Σ ?Γ) =>
   match goal with
-    | [ H : typing Σ Γ _ _ |- _ ] => apply (typing_wf_local H)
+  | [ H : typing Σ Γ _ _ |- _ ] => apply (typing_wf_local H)
   end : pcuic.
 
-Ltac pcuic := try solve [ intuition typeclasses eauto with pcuic ].
+  Ltac pcuic := try solve [ intuition typeclasses eauto with pcuic ].
 
-Definition weaken_env_prop_full
-           (P : global_env_ext -> context -> term -> term -> Type) :=
-  forall Σ Σ', wf Σ' -> extends Σ Σ' -> forall Γ t T, P Σ Γ t T -> P Σ' Γ t T.
+  Definition weaken_env_prop_full
+             (P : global_env_ext -> context -> term -> term -> Type) :=
+    forall Σ (Σ' : global_env_ext), wf Σ' -> extends Σ.1 Σ'.1 -> forall Γ t T, P Σ Γ t T -> P Σ' Γ t T.
 
-Lemma isWfArity_or_Type_weaken_full : weaken_env_prop_full (fun Σ Γ t T => isWfArity_or_Type Σ Γ T).
-Proof.
-  red. intros.
-  destruct X1. left. destruct i as [ctx [s [Heq Hs]]].
-  exists ctx, s. pcuic. right. destruct i as [u Hu]; exists u; pcuic.
-  unshelve eapply (weaken_env_prop_typing _ _ _ X0 _ _ (Some (tSort u))); eauto.
-Qed.
-Hint Resolve isWfArity_or_Type_weaken_full : pcuic.
+  Lemma isWfArity_or_Type_weaken_full : weaken_env_prop_full (fun Σ Γ t T => isWfArity_or_Type Σ Γ T).
+  Proof.
+    red. intros.
+    destruct X1. left. destruct i as [ctx [s [Heq Hs]]].
+    exists ctx, s. split; auto. pcuic.
+    apply exists
+    right. destruct i as [u Hu]; exists u; pcuic.
+    unshelve eapply (weaken_env_prop_typing _ _ _ X0 _ _ (Some (tSort u))); eauto.
+  Qed.
+  Hint Resolve isWfArity_or_Type_weaken_full : pcuic.
 
-Lemma isWfArity_or_Type_weaken :
- weaken_env_prop
-   (lift_typing (fun Σ Γ (_ T : term) => isWfArity_or_Type Σ Γ T)).
-Proof.
-  red. intros. unfold lift_typing in *. destruct T. now eapply isWfArity_or_Type_weaken_full.
-  destruct X1 as [s Hs]; exists s. now eapply isWfArity_or_Type_weaken_full.
-Qed.
-Hint Resolve isWfArity_or_Type_weaken : pcuic.
+  Lemma isWfArity_or_Type_weaken :
+    weaken_env_prop
+      (lift_typing (fun Σ Γ (_ T : term) => isWfArity_or_Type Σ Γ T)).
+  Proof.
+    red. intros. unfold lift_typing in *. destruct T. now eapply isWfArity_or_Type_weaken_full.
+    destruct X1 as [s Hs]; exists s. now eapply isWfArity_or_Type_weaken_full.
+  Qed.
+  Hint Resolve isWfArity_or_Type_weaken : pcuic.
 
-(** TODO: Universe instances *)
-Lemma isWfArity_or_Type_subst_instance:
-  forall (Σ : global_env_ext) (Γ : context) (u : list Level.t) (ty : term), wf_local Σ Γ ->
-    isWfArity_or_Type Σ [] ty -> isWfArity_or_Type Σ Γ (PCUICUnivSubst.subst_instance_constr u ty).
-Proof.
-  intros Σ Γ u ty wfΓ H.
-  destruct H as [[ctx [s [Heq Hs]]]|].
-  - left.
-    exists ctx, s. split; pcuic.
-Admitted.
+  (** TODO: Universe instances *)
+  Lemma isWfArity_or_Type_subst_instance:
+    forall (Σ : global_env_ext) (Γ : context) (u : list Level.t) (ty : term), wf_local Σ Γ ->
+                                                                              isWfArity_or_Type Σ [] ty -> isWfArity_or_Type Σ Γ (PCUICUnivSubst.subst_instance_constr u ty).
+  Proof.
+    intros Σ Γ u ty wfΓ H.
+    destruct H as [[ctx [s [Heq Hs]]]|].
+    - left.
+      exists ctx, s. split; pcuic.
+  Admitted.
 
-Lemma invert_type_mkApps Σ Γ f fty u T :
-  Σ ;;; Γ |- mkApps f u : T ->
-  (* Looks mutual with validity! *)
-  Σ ;;; Γ |- f : fty -> isWfArity_or_Type Σ Γ fty ->
-  { T' & { U & ((Σ ;;; Γ |- f : T') * (typing_spine Σ Γ T' u U) * (Σ ;;; Γ |- U <= T))%type } }.
-Proof.
-  induction u in f, fty, T |- *. simpl. intros. exists T, T. intuition auto. constructor.
-  intros Hf Hty. simpl in Hty.
-  specialize (IHu _ fty _ Hf) as [T' [U' [[H' H''] H''']]].
-  simpl in Hf.
-  econstructor.
+  Lemma invert_type_mkApps Σ Γ f fty u T :
+    Σ ;;; Γ |- mkApps f u : T ->
+                            (* Looks mutual with validity! *)
+                            Σ ;;; Γ |- f : fty -> isWfArity_or_Type Σ Γ fty ->
+                                           { T' & { U & ((Σ ;;; Γ |- f : T') * (typing_spine Σ Γ T' u U) * (Σ ;;; Γ |- U <= T))%type } }.
+  Proof.
+    induction u in f, fty, T |- *. simpl. intros. exists T, T. intuition auto. constructor.
+    intros Hf Hty. simpl in Hty.
+    specialize (IHu _ fty _ Hf) as [T' [U' [[H' H''] H''']]].
+    simpl in Hf.
+    econstructor.
 
-Admitted.
-(*   eapply invert_type_App in H' as (fA & fB & fna & Hf). intuition. *)
-(*   exists (tProd fna fA fB), U'. intuition auto. *)
-(*   econstructor. *)
-(*   exists T', U'. split; auto. split; auto. *)
-(*   eapply cumul_trans; eauto. *)
-(* Qed. *)
+  Admitted.
+  (*   eapply invert_type_App in H' as (fA & fB & fna & Hf). intuition. *)
+  (*   exists (tProd fna fA fB), U'. intuition auto. *)
+  (*   econstructor. *)
+  (*   exists T', U'. split; auto. split; auto. *)
+  (*   eapply cumul_trans; eauto. *)
+  (* Qed. *)
 
-Theorem validity :
-  env_prop (fun Σ Γ t T => isWfArity_or_Type Σ Γ T).
-Proof.
+  Theorem validity :
+    env_prop (fun Σ Γ t T => isWfArity_or_Type Σ Γ T).
+  Proof.
 
-  apply typing_ind_env; intros; rename_all_hyps.
+    apply typing_ind_env; intros; rename_all_hyps.
 
-  - destruct (nth_error_All_local_env_over heq_nth_error X) as [HΓ' Hd].
-    destruct decl as [na [b|] ty]; cbn -[skipn] in *.
-    + eapply isWfArity_or_Type_lift; eauto. clear HΓ'; now apply nth_error_Some_length in heq_nth_error.
-    + destruct lookup_wf_local_decl; cbn -[skipn] in *.
-      destruct o. right. exists x0. simpl in Hd.
-      rewrite <- (firstn_skipn (S n) Γ).
-      assert (S n = #|firstn (S n) Γ|).
-      { apply nth_error_Some_length in heq_nth_error. rewrite firstn_length_le; auto with arith. }
-      rewrite {3}H.
-      apply (weakening Σ (skipn (S n) Γ) (firstn (S n) Γ) ty (tSort x0)); eauto with wf.
-      unfold app_context. now rewrite (firstn_skipn (S n) Γ).
+    - destruct (nth_error_All_local_env_over heq_nth_error X) as [HΓ' Hd].
+      destruct decl as [na [b|] ty]; cbn -[skipn] in *.
+      + eapply isWfArity_or_Type_lift; eauto. clear HΓ'; now apply nth_error_Some_length in heq_nth_error.
+      + destruct lookup_wf_local_decl; cbn -[skipn] in *.
+        destruct o. right. exists x0. simpl in Hd.
+        rewrite <- (firstn_skipn (S n) Γ).
+        assert (S n = #|firstn (S n) Γ|).
+        { apply nth_error_Some_length in heq_nth_error. rewrite firstn_length_le; auto with arith. }
+        rewrite {3}H.
+        apply (weakening Σ (skipn (S n) Γ) (firstn (S n) Γ) ty (tSort x0)); eauto with wf.
+        unfold app_context. now rewrite (firstn_skipn (S n) Γ).
 
-  - (* Universe *) left. exists [], (Universe.super l). split; auto.
-  - (* Product *) left. eexists [], _. split; eauto. simpl. reflexivity.
-  - (* Lambda *)
-    destruct X3.
-    + left. destruct i as [ctx [s [Heq Hs]]].
-      red. simpl. pose proof (PCUICClosed.destArity_spec [] bty).
-      rewrite Heq in H. simpl in H. subst bty. clear Heq.
-      eexists _, s. split; auto.
-      * rewrite destArity_it_mkProd_or_LetIn. simpl. reflexivity.
-      * apply All_local_env_app_inv; split; auto.
-        apply All_local_env_app_inv; split; auto.
-        -- repeat constructor.
-           simpl. now exists s1.
-        -- apply All_local_env_app in Hs. unfold snoc.
-           intuition auto. clear -b0.
-           induction b0; constructor; eauto.
-           ++ destruct t1 as [u Hu]. exists u.
-              rewrite app_context_assoc. apply Hu.
-           ++ simpl in t1 |- *.
-              rewrite app_context_assoc. apply t1.
-           ++ simpl in t2.
-              rewrite app_context_assoc. apply t2.
-    + destruct i as [u Hu].
-      right. exists (Universe.sort_of_product s1 u); constructor; auto.
+    - (* Universe *) left. exists [], (Universe.super l). split; auto.
+    - (* Product *) left. eexists [], _. split; eauto. simpl. reflexivity.
+    - (* Lambda *)
+      destruct X3.
+      + left. destruct i as [ctx [s [Heq Hs]]].
+        red. simpl. pose proof (PCUICClosed.destArity_spec [] bty).
+        rewrite Heq in H. simpl in H. subst bty. clear Heq.
+        eexists _, s. split; auto.
+        * rewrite destArity_it_mkProd_or_LetIn. simpl. reflexivity.
+        * apply All_local_env_app_inv; split; auto.
+          apply All_local_env_app_inv; split; auto.
+          -- repeat constructor.
+             simpl.
+             exists s1; easy.
+          -- apply All_local_env_app in Hs. unfold snoc.
+             intuition auto. clear -b0.
+             induction b0; constructor; eauto.
+             ++ destruct t1 as [u Hu]. exists u.
+                rewrite app_context_assoc. apply Hu.
+             ++ simpl in t1 |- *.
+                rewrite app_context_assoc. apply t1.
+             ++ simpl in t2.
+                rewrite app_context_assoc. apply t2.
+      + destruct i as [u Hu].
+        right. exists (Universe.sort_of_product s1 u); constructor; auto.
 
-  - (* Let *)
-    destruct X5.
-    + left. destruct i as [ctx [s [Heq Hs]]].
-      eexists _, s.
-      simpl. split; auto.
-      pose proof (PCUICClosed.destArity_spec [] b'_ty).
-      rewrite Heq in H. simpl in H. subst b'_ty.
-      rewrite destArity_it_mkProd_or_LetIn. simpl.
-      reflexivity. rewrite app_context_assoc. simpl.
-      apply All_local_env_app_inv; split; eauto with wf.
-      apply All_local_env_app in Hs as [Hp Hs].
-      apply Hs.
-    + right.
-      destruct i as [u Hu]. exists u.
-      econstructor.
-      eapply type_LetIn; eauto. left. exists [], u; intuition eauto with wf.
-      eapply cumul_alt. exists (tSort u), (tSort u); intuition auto.
-      apply red1_red; repeat constructor.
+    - (* Let *)
+      destruct X5.
+      + left. destruct i as [ctx [s [Heq Hs]]].
+        eexists _, s.
+        simpl. split; auto.
+        pose proof (PCUICClosed.destArity_spec [] b'_ty).
+        rewrite Heq in H. simpl in H. subst b'_ty.
+        rewrite destArity_it_mkProd_or_LetIn. simpl.
+        reflexivity. rewrite app_context_assoc. simpl.
+        apply All_local_env_app_inv; split; eauto with wf.
+        apply All_local_env_app in Hs as [Hp Hs].
+        apply Hs.
+      + right.
+        destruct i as [u Hu]. exists u.
+        econstructor.
+        eapply type_LetIn; eauto. left. exists [], u; intuition eauto with wf.
+        eapply cumul_alt. exists (tSort u), (tSort u); intuition auto.
+        apply red1_red; repeat constructor.
 
-  - (* Application *)
-    destruct X1 as [[ctx [s [Heq Hs]]]|].
-    simpl in Heq. pose proof (PCUICClosed.destArity_spec ([],, vass na A) B).
-    rewrite Heq in H.
-    simpl in H. unfold mkProd_or_LetIn in H. simpl in H.
-    destruct ctx using rev_ind; noconf H.
-    simpl in H. rewrite it_mkProd_or_LetIn_app in H. simpl in H.
-    destruct x as [na' [b|] ty]; noconf H.
-    left. eexists _, s. split.
-    unfold subst1. rewrite subst_it_mkProd_or_LetIn.
-    rewrite destArity_it_mkProd_or_LetIn. simpl. reflexivity.
-    rewrite app_context_nil_l. apply All_local_env_app_inv; intuition auto.
-    apply All_local_env_app in Hs as [wf'Γ wfctx].
-    apply All_local_env_app in wfctx as [wfd wfctx].
-    eapply All_local_env_subst; eauto. simpl; intros.
-    destruct T; simpl in *.
-    + rewrite Nat.add_0_r. eapply substitution_alt; eauto. constructor. constructor.
-      2: simpl; eauto; now rewrite app_context_assoc in X0.
-      now rewrite subst_empty.
-    + rewrite Nat.add_0_r. destruct X0 as [u' Hu']. exists u'.
-      eapply (substitution_alt _ _ _ _ _ _ (tSort u')); eauto. constructor. constructor.
-      2: simpl; eauto; now rewrite app_context_assoc in Hu'.
-      now rewrite subst_empty.
-    + right.
-      destruct i as [u' Hu']. exists u'.
-      eapply (substitution0 _ _ na _ _ _ (tSort u')); eauto.
-      apply inversion_Prod in Hu' as [na' [s1 [s2 Hs]]]. intuition.
-      eapply type_Conv; pcuic.
-      eapply (weakening_cumul Σ Γ [] [vass na A]) in b; pcuic.
-      simpl in b. eapply cumul_trans. 2:eauto.
-      constructor. constructor. simpl. apply leq_universe_product.
+    - (* Application *)
+      destruct X1 as [[ctx [s [Heq Hs]]]|].
+      simpl in Heq. pose proof (PCUICClosed.destArity_spec ([],, vass na A) B).
+      rewrite Heq in H.
+      simpl in H. unfold mkProd_or_LetIn in H. simpl in H.
+      destruct ctx using rev_ind; noconf H.
+      simpl in H. rewrite it_mkProd_or_LetIn_app in H. simpl in H.
+      destruct x as [na' [b|] ty]; noconf H.
+      left. eexists _, s. split.
+      unfold subst1. rewrite subst_it_mkProd_or_LetIn.
+      rewrite destArity_it_mkProd_or_LetIn. simpl. reflexivity.
+      rewrite app_context_nil_l. apply All_local_env_app_inv; intuition auto.
+      apply All_local_env_app in Hs as [wf'Γ wfctx].
+      apply All_local_env_app in wfctx as [wfd wfctx].
+      eapply All_local_env_subst; eauto. simpl; intros.
+      destruct T; simpl in *.
+      + rewrite Nat.add_0_r. eapply substitution_alt; eauto. constructor. constructor.
+        2: simpl; eauto; now rewrite app_context_assoc in X0.
+        now rewrite subst_empty.
+      + rewrite Nat.add_0_r. destruct X0 as [u' Hu']. exists u'.
+        eapply (substitution_alt _ _ _ _ _ _ (tSort u')); eauto. constructor. constructor.
+        2: simpl; eauto; now rewrite app_context_assoc in Hu'.
+        now rewrite subst_empty.
+      + right.
+        destruct i as [u' Hu']. exists u'.
+        eapply (substitution0 _ _ na _ _ _ (tSort u')); eauto.
+        apply inversion_Prod in Hu' as [na' [s1 [s2 Hs]]]. intuition.
+        eapply type_Conv; pcuic.
+        eapply (weakening_cumul Σ Γ [] [vass na A]) in b; pcuic.
+        simpl in b. eapply cumul_trans. 2:eauto.
+        constructor. constructor. simpl. apply leq_universe_product.
 
-  - eapply declared_constant_inv in H; pcuic.
-    destruct decl as [ty [b|] univs]. red in H. simpl in *.
-    apply isWfArity_or_Type_subst_instance; pcuic.
-    repeat red in H; simpl in *.
-    apply isWfArity_or_Type_subst_instance; pcuic.
-    destruct H.
-    (* TODO: Fix Forall_decls_typing same way as local environments *)
-    admit.
-  - admit.
-  - admit.
+    - eapply declared_constant_inv in H; pcuic.
+      destruct decl as [ty [b|] univs]. red in H. simpl in *.
+      apply isWfArity_or_Type_subst_instance; pcuic.
+      repeat red in H; simpl in *.
+      apply isWfArity_or_Type_subst_instance; pcuic.
+      destruct H.
+      (* TODO: Fix Forall_decls_typing same way as local environments *)
+      admit.
+    - admit.
+    - admit.
 
-  - (* Case *)
-    right. red.
-    destruct X2.
-    + destruct i as [ctx [s [Heq Hs]]].
-      exists s.
-      unfold check_correct_arity in *.
-      assert (ctx = pctx). admit. (* WF of cases *)
-      subst ctx.
-      pose proof (PCUICClosed.destArity_spec [] pty). rewrite Heq in H.
-      simpl in H. subst pty.
-      assert (#|args| = #|pctx|). admit. (* WF of case *)
-      eapply type_mkApps. eauto.
-      destruct X4. destruct i as [ctx' [s' [Heq' Hs']]].
-      elimtype False.
-      { clear -Heq'.
-        revert Heq'.
-        assert (destArity [] (tInd ind u) = None) by reflexivity.
-        revert H.
-        generalize (tInd ind u). clear. induction args.
-        intros. simpl in Heq'. congruence.
-        intros. unshelve eapply (IHargs _ _ Heq').
-        reflexivity. }
-      destruct i as [si Hi].
-      eapply (invert_type_mkApps _ _ (tInd ind u)) in Hi; pcuic.
-      2:{ econstructor; eauto. admit. (* universes *) }
-      2:{ admit. }
-      (* Looks ok *)
+    - (* Case *)
+      right. red.
+      destruct X2.
+      + destruct i as [ctx [s [Heq Hs]]].
+        exists s.
+        unfold check_correct_arity in *.
+        assert (ctx = pctx). admit. (* WF of cases *)
+        subst ctx.
+        pose proof (PCUICClosed.destArity_spec [] pty). rewrite Heq in H.
+        simpl in H. subst pty.
+        assert (#|args| = #|pctx|). admit. (* WF of case *)
+        eapply type_mkApps. eauto.
+        destruct X4. destruct i as [ctx' [s' [Heq' Hs']]].
+        elimtype False.
+        { clear -Heq'.
+          revert Heq'.
+          assert (destArity [] (tInd ind u) = None) by reflexivity.
+          revert H.
+          generalize (tInd ind u). clear. induction args.
+          intros. simpl in Heq'. congruence.
+          intros. unshelve eapply (IHargs _ _ Heq').
+          reflexivity. }
+        destruct i as [si Hi].
+        eapply (invert_type_mkApps _ _ (tInd ind u)) in Hi; pcuic.
+        2:{ econstructor; eauto. admit. (* universes *) }
+        2:{ admit. }
+        (* Looks ok *)
+        admit.
+
+      + destruct i as [ui Hi]. exists ui.
+        admit. (* Same idea *)
+
+    - (* Proj *)
+      right.
       admit.
 
-    + destruct i as [ui Hi]. exists ui.
-      admit. (* Same idea *)
+    - admit. (* Fix *)
+    - admit. (* CoFix *)
 
-  - (* Proj *)
-    right.
-    admit.
-
-  - admit. (* Fix *)
-  - admit. (* CoFix *)
-
-  - (* Conv *)
-    destruct X2. red in i. left. exact (projT1 i).
-    right. destruct s as [u [Hu _]]. now exists u.
-Admitted.
+    - (* Conv *)
+      destruct X2. red in i. left. exact (projT1 i).
+      right. destruct s as [u [Hu _]]. now exists u.
+  Admitted.
